Add list of type variables in type inferencer

TypeInferencer.v
@@ -12,88 +12,88 @@ Require Import AST.
 Require Import Maps.
 
 
-Inductive typeinf : t_env -> nat -> t_expr -> (nat * t_type * constr) % type -> Prop :=
+Inductive typeinf : t_env -> nat -> t_expr -> (nat * t_type * constr * list id) % type -> Prop :=
   (* ENum *)
   (* EBool *)
   (* EVar *)
   | TI_Num: forall env n fv,
-    typeinf env fv (ENum n) (fv, TNum, [])
+    typeinf env fv (ENum n) (fv, TNum, [], [])
   | TI_Bool: forall env b fv,
-    typeinf env fv (EBool b) (fv, TBool, [])
+    typeinf env fv (EBool b) (fv, TBool, [], [])
   | TI_Var: forall env x fv T,
-    env x = Some T -> typeinf env fv (EVar x) (fv, T, [])
+    env x = Some T -> typeinf env fv (EVar x) (fv, T, [], [])
 
   (* EIf *)
   | TI_If:
     forall env fv
-      c c_fv c_C c_T
-      e1 e1_fv e1_C e1_T
-      e2 e2_fv e2_C e2_T,
-    typeinf env fv c (c_fv, c_T, c_C) ->
-    typeinf env c_fv  e1 (e1_fv, e1_T, e1_C) ->
-    typeinf env e1_fv  e2 (e2_fv, e2_T, e2_C) ->
-    typeinf env fv (EIf c e1 e2) (e2_fv, e1_T, e2_C ++ e1_C ++ c_C ++ [(e1_T, e2_T); (c_T, TBool)])
+      c c_fv c_C c_T c_X
+      e1 e1_fv e1_C e1_T e1_X
+      e2 e2_fv e2_C e2_T e2_X,
+    typeinf env fv c (c_fv, c_T, c_C, c_X) ->
+    typeinf env c_fv  e1 (e1_fv, e1_T, e1_C, e1_X) ->
+    typeinf env e1_fv  e2 (e2_fv, e2_T, e2_C, e2_X) ->
+    typeinf env fv (EIf c e1 e2) (e2_fv, e1_T, e2_C ++ e1_C ++ c_C ++ [(e1_T, e2_T); (c_T, TBool)], e2_X ++ e1_X ++ c_X)
 
   (* EFun *)
   | TI_Fun:
     forall env fv
-      x x_T e e_fv e_C e_T,
-    typeinf (update env x x_T) fv  e (e_fv, e_T, e_C) ->
-    typeinf env fv (EFun x x_T e) (e_fv, (TFun x_T e_T), e_C)
+      x x_T e e_fv e_C e_T e_X,
+    typeinf (update env x x_T) fv e (e_fv, e_T, e_C, e_X) ->
+    typeinf env fv (EFun x x_T e) (e_fv, (TFun x_T e_T), e_C, e_X)
 
   (* ECall *)
   | TI_Call:
     forall env fv
-      f f_fv f_C f_T
-      e e_fv e_C e_T,
-    typeinf env fv f (f_fv, f_T, f_C) ->
-    typeinf env f_fv e (e_fv, e_T, e_C) ->
-    typeinf env fv (ECall f e) (e_fv + 1, TVar (Id e_fv), e_C ++ f_C ++ [(f_T, TFun e_T (TVar (Id e_fv)))])
+      f f_fv f_C f_T f_X
+      e e_fv e_C e_T e_X,
+    typeinf env fv f (f_fv, f_T, f_C, f_X) ->
+    typeinf env f_fv e (e_fv, e_T, e_C, e_X) ->
+    typeinf env fv (ECall f e) (e_fv + 1, TVar (Id e_fv), e_C ++ f_C ++ [(f_T, TFun e_T (TVar (Id e_fv)))], e_X ++ f_X ++ [Id e_fv])
 
   (* ECons *)
   | TI_Cons:
     forall env fv
-      hd hd_fv hd_C hd_T
-      tl tl_fv tl_C tl_T,
-    typeinf env fv hd (hd_fv, hd_T, hd_C) ->
-    typeinf env hd_fv tl (tl_fv, tl_T, tl_C) ->
-    typeinf env fv (ECons hd tl) (tl_fv, TList hd_T, tl_C ++ hd_C ++ [(tl_T, TList hd_T)])
+      hd hd_fv hd_C hd_T hd_X
+      tl tl_fv tl_C tl_T tl_X,
+    typeinf env fv hd (hd_fv, hd_T, hd_C, hd_X) ->
+    typeinf env hd_fv tl (tl_fv, tl_T, tl_C, tl_X) ->
+    typeinf env fv (ECons hd tl) (tl_fv, TList hd_T, tl_C ++ hd_C ++ [(tl_T, TList hd_T)], tl_X ++ hd_X)
 
   (* ENil *)
   | TI_Nil:
     forall env T fv,
-    typeinf env fv (ENil T) (fv, TList T, [])
+    typeinf env fv (ENil T) (fv, TList T, [], [])
 
   (* EBinop *)
   | TI_Binop_nnn:
     forall env fv op
-      e1 e1_fv e1_C e1_T
-      e2 e2_fv e2_C e2_T,
-    typeinf env fv e1 (e1_fv, e1_T, e1_C) ->
-    typeinf env e1_fv e2 (e2_fv, e2_T, e2_C) ->
+      e1 e1_fv e1_C e1_T e1_X
+      e2 e2_fv e2_C e2_T e2_X,
+    typeinf env fv e1 (e1_fv, e1_T, e1_C, e1_X) ->
+    typeinf env e1_fv e2 (e2_fv, e2_T, e2_C, e2_X) ->
     op = OpPlus \/
     op = OpMinus ->
-    typeinf env fv (EBinop op e1 e2) (e2_fv, TNum, e2_C++ e1_C ++ [(e2_T, TNum); (e1_T, TNum)])
+    typeinf env fv (EBinop op e1 e2) (e2_fv, TNum, e2_C++ e1_C ++ [(e2_T, TNum); (e1_T, TNum)], e2_X ++ e1_X)
 
   | TI_Binop_nnb:
     forall env fv op
-      e1 e1_fv e1_C e1_T
-      e2 e2_fv e2_C e2_T,
-    typeinf env fv e1 (e1_fv, e1_T, e1_C) ->
-    typeinf env e1_fv e2 (e2_fv, e2_T, e2_C) ->
+      e1 e1_fv e1_C e1_T e1_X
+      e2 e2_fv e2_C e2_T e2_X,
+    typeinf env fv e1 (e1_fv, e1_T, e1_C, e1_X) ->
+    typeinf env e1_fv e2 (e2_fv, e2_T, e2_C, e2_X) ->
     op = OpEq \/
     op = OpNeq ->
-    typeinf env fv (EBinop op e1 e2) (e2_fv, TBool, e2_C++ e1_C ++ [(e2_T, TNum); (e1_T, TNum)])
+    typeinf env fv (EBinop op e1 e2) (e2_fv, TBool, e2_C++ e1_C ++ [(e2_T, TNum); (e1_T, TNum)], e2_X ++ e1_X)
 
   | TI_Binop_bbb:
     forall env fv op
-      e1 e1_fv e1_C e1_T
-      e2 e2_fv e2_C e2_T,
-    typeinf env fv e1 (e1_fv, e1_T, e1_C) ->
-    typeinf env e1_fv e2 (e2_fv, e2_T, e2_C) ->
+      e1 e1_fv e1_C e1_T e1_X
+      e2 e2_fv e2_C e2_T e2_X,
+    typeinf env fv e1 (e1_fv, e1_T, e1_C, e1_X) ->
+    typeinf env e1_fv e2 (e2_fv, e2_T, e2_C, e2_X) ->
     op = OpAnd \/
     op = OpOr ->
-    typeinf env fv (EBinop op e1 e2) (e2_fv, TBool, e2_C++ e1_C ++ [(e2_T, TBool); (e1_T, TBool)]).
+    typeinf env fv (EBinop op e1 e2) (e2_fv, TBool, e2_C++ e1_C ++ [(e2_T, TBool); (e1_T, TBool)], e2_X ++ e1_X).
 
 Fixpoint app_sub_to_type (s : substs) (t : t_type) : t_type :=
   match t with
@@ -124,7 +124,7 @@ Fixpoint app_sub_to_expr (s : substs) (e : t_expr) : t_expr :=
       ENil (app_sub_to_type s T)
   end.
 
-Definition app_sub_to_env (s : substs) (env : t_env) : id -> option t_type :=
+Definition app_sub_to_env (s : substs) (env : t_env) : substs :=
   (fun i =>
     match env i with
       | Some T => Some (app_sub_to_type s T)
